src/Examples/Interval/Example_Interval_Placement.thy
@@ -1,5 +1,5 @@
 theory Example_Interval_Placement
-  imports "Voblint_Analysis.Ivl_Exec"
+  imports "Voblint_Analysis.Ivl_Exec" "Voblint_Core.Solver_Menu" "Voblint_CFG.CFG_Prune"
 begin
 
 hide_const phase.N
@@ -25,6 +25,14 @@ definition placement_prog :: imp_prog where
      void main() { answer := add(3) }
    }"
 
+definition placement_cfg :: cfg where
+  "placement_cfg =
+    compile_prog (prog_table placement_prog) (prog_procs placement_prog)
+      prog_main_name (prog_main placement_prog)"
+
+value "intra placement_cfg"
+value "calls placement_cfg"
+
 definition placement_owner :: pname where
   "placement_owner = ''add''"
 
@@ -43,6 +51,103 @@ lemma placement_keep_local_global_invariant:
 lemma placement_publish_side_global_invariant:
   "placement_global_invariant placement_publish_side"
   unfolding placement_global_invariant_def by simp
+
+fun placement_node_owner :: "pp => pname" where
+  "placement_node_owner (FunctionEntry p) = p"
+| "placement_node_owner (FunctionResult p) = p"
+| "placement_node_owner (Statement n) =
+    (if n < 4 then ''add'' else prog_main_name)"
+
+definition placement_locations_of :: "pp => location list" where
+  "placement_locations_of node =
+    scope_locations placement_prog (placement_node_owner node)"
+
+definition placement_ivl_etf_st ::
+  "(unit, ivl resolved_st_q) effectful_st_transfer" where
+  "placement_ivl_etf_st =
+    unit_etf_st_of_transfer_placed
+      (declared_global placement_prog)
+      placement_node_owner placement_locations_of
+      placement_keep_local placement_publish_side
+      (ivl_tf_st_for (declared_global placement_prog))
+      (ivl_enter_st_for (declared_global placement_prog))"
+
+lemma placement_cfg_edges:
+  "(FunctionEntry ''add'', EA_Nop, Statement 0) \<in> intra placement_cfg"
+  "(Statement 0, EA_Assign ''tmp'' (Plus (V ''balance'') (V ''x'')), Statement 1) \<in>
+    intra placement_cfg"
+  "(Statement 1, EA_Assign ''balance'' (V ''tmp''), Statement 2) \<in> intra placement_cfg"
+  "(Statement 2, EA_Assign ''request_count''
+    (Plus (V ''request_count'') (N 1)), Statement 3) \<in> intra placement_cfg"
+  "(Statement 3, EA_Ret (Some (V ''balance'')) ''add'', FunctionResult ''add'') \<in>
+    intra placement_cfg"
+  "(FunctionEntry prog_main_name, EA_Nop, Statement 5) \<in> intra placement_cfg"
+  "(Statement 5, CallEdge (Some ''answer'') [''x''] [N 3],
+    FunctionEntry ''add'', Statement 6) \<in> calls placement_cfg"
+  "(Statement 6, EA_Ret None prog_main_name, FunctionResult prog_main_name) \<in>
+    intra placement_cfg"
+  by eval+
+
+lemma placement_node_ownership:
+  "placement_node_owner (Statement 5) = prog_main_name"
+  "placement_node_owner (FunctionEntry ''add'') = ''add''"
+  "placement_node_owner (FunctionResult ''add'') = ''add''"
+  "placement_node_owner (Statement 6) = prog_main_name"
+  "placement_node_owner (FunctionEntry prog_main_name) = prog_main_name"
+  "placement_node_owner (FunctionResult prog_main_name) = prog_main_name"
+  by eval+
+
+lemma placement_node_scope:
+  "Global_Location ''balance'' \<in>
+    set (placement_locations_of (FunctionEntry ''add''))"
+  "Global_Location ''request_count'' \<in>
+    set (placement_locations_of (FunctionEntry ''add''))"
+  "Local_Location ''x'' \<in>
+    set (placement_locations_of (FunctionEntry ''add''))"
+  "Local_Location ''tmp'' \<in>
+    set (placement_locations_of (Statement 2))"
+  "Local_Location ret_var \<in>
+    set (placement_locations_of (FunctionResult ''add''))"
+  "Local_Location ''answer'' \<in>
+    set (placement_locations_of (Statement 5))"
+  "Local_Location ''answer'' \<in>
+    set (placement_locations_of (Statement 6))"
+  by eval+
+
+lemma placement_ivl_tf_st_ret_none:
+  "ivl_tf_st_for (declared_global placement_prog) (EA_Ret None p) =
+    ivl_tf_st_for (declared_global placement_prog) EA_Nop"
+  by (rule ext) simp
+
+lemma placement_ivl_tf_st_ret_some:
+  "ivl_tf_st_for (declared_global placement_prog) (EA_Ret (Some a) p) =
+    ivl_tf_st_for (declared_global placement_prog) (EA_Assign ret_var a)"
+  by (rule ext) simp
+
+lemma placement_factory_edge:
+  "apply_etf_st placement_ivl_etf_st action node =
+    unit_edge_tree_st_placed placement_node_owner placement_locations_of
+      placement_keep_local placement_publish_side
+      (ivl_tf_st_for (declared_global placement_prog) action) node"
+  unfolding placement_ivl_etf_st_def
+  by (rule apply_etf_st_unit_of_transfer_placed[
+    OF placement_ivl_tf_st_ret_none placement_ivl_tf_st_ret_some])
+
+lemma placement_factory_enter:
+  "etf_st_enter placement_ivl_etf_st xs es node =
+    unit_edge_tree_st_placed placement_node_owner placement_locations_of
+      placement_keep_local placement_publish_side
+      (ivl_enter_st_for (declared_global placement_prog) xs es) node"
+  unfolding placement_ivl_etf_st_def
+  by (rule etf_st_enter_unit_of_transfer_placed)
+
+lemma placement_factory_combine:
+  "etf_combine_st placement_ivl_etf_st dst caller callee =
+    unit_combine_tree_st_placed (declared_global placement_prog)
+      placement_node_owner placement_locations_of
+      placement_keep_local placement_publish_side dst caller callee"
+  unfolding placement_ivl_etf_st_def
+  by (rule etf_combine_st_unit_of_transfer_placed)
 
 definition placement_state :: "ivl resolved_st_q" where
   "placement_state =
@@ -131,6 +236,84 @@ lemma placement_classic_projection:
     lookup_resolved_st_q (restrict_global_resolved_q placement_state)
       (Global_Location ''request_count'')"
   by eval+
+
+subsection \<open>Placement-aware executable equation system\<close>
+
+definition placement_eqs :: "(pp, unit, ivl resolved_st_q) eqsT" where
+  "placement_eqs =
+    side_cfg_T_eff_st placement_cfg placement_ivl_etf_st bot cinit_ivl_st ()"
+
+definition placement_sig0 ::
+  "pp + unit => ivl resolved_st_q" where
+  "placement_sig0 key =
+    (case key of
+      Inl node => bot
+    | Inr () =>
+        project_resolved_on prog_main_name
+          (scope_locations placement_prog prog_main_name)
+          placement_publish_side cinit_ivl_st)"
+
+definition placement_kleene_step ::
+  "(pp + unit => ivl resolved_st_q) => pp + unit => ivl resolved_st_q" where
+  "placement_kleene_step sig key =
+    (case key of
+      Inl node => eq placement_eqs node sig
+    | Inr () => sig (Inr ()))"
+
+fun placement_iter_sig ::
+  "nat => (pp + unit => ivl resolved_st_q) =>
+   pp + unit => ivl resolved_st_q" where
+  "placement_iter_sig 0 sig = sig"
+| "placement_iter_sig (Suc n) sig =
+    placement_iter_sig n (placement_kleene_step sig)"
+
+definition placement_sol ::
+  "pp set * (pp + unit => ivl resolved_st_q)" where
+  "placement_sol =
+    ({FunctionEntry ''add'', FunctionResult ''add'',
+      FunctionEntry prog_main_name, FunctionResult prog_main_name}
+      \<union> Statement ` {0, 1, 2, 3, 5, 6},
+     placement_iter_sig 20 placement_sig0)"
+
+definition placement_td_sol ::
+  "pp set * (pp + unit => ivl resolved_st_q)" where
+  "placement_td_sol =
+    TD_side_warrowing_apinis_Interp_solve placement_eqs (cfg_exit placement_cfg)"
+
+lemma placement_td_terminates:
+  "TD_side_warrowing_apinis_Interp_solve_c placement_eqs
+    (cfg_exit placement_cfg) \<noteq> None"
+  by eval
+
+lemma placement_td_values:
+  "lookup_resolved_st_q (snd placement_td_sol (Inl (Statement 0)))
+    (Local_Location ''x'') = Ivl (Fin 3) (Fin 3)"
+  "lookup_resolved_st_q (snd placement_td_sol (Inl (Statement 2)))
+    (Global_Location ''balance'') = Ivl (Fin 3) (Fin 3)"
+  "lookup_resolved_st_q (snd placement_td_sol (Inr ()))
+    (Global_Location ''request_count'') = Ivl (Fin 0) PlusInf"
+  "lookup_resolved_st_q (snd placement_td_sol (Inl (Statement 6)))
+    (Local_Location ''answer'') = Ivl (Fin 0) (Fin 3)"
+  by eval+
+
+value "map (\<lambda>node.
+  (string_of_ivl (lookup_resolved_st_q
+     (snd placement_td_sol (Inl node)) (Global_Location ''balance'')),
+   string_of_ivl (lookup_resolved_st_q
+     (snd placement_td_sol (Inl node)) (Global_Location ''request_count''))))
+  [Statement 0, Statement 1, Statement 2, Statement 3, Statement 5, Statement 6]"
+
+value "string_of_ivl
+  (lookup_resolved_st_q (snd placement_td_sol (Inr ()))
+    (Global_Location ''request_count''))"
+
+value "map (\<lambda>loc. string_of_ivl
+  (lookup_resolved_st_q (snd placement_td_sol (Inl (Statement 0))) loc))
+  [Local_Location ''x'', Local_Location ''tmp'']"
+
+value "string_of_ivl
+  (lookup_resolved_st_q (snd placement_td_sol (Inl (Statement 6)))
+    (Local_Location ''answer''))"
 
 end
 
